theories/language/adequacy.v
@@ -17,13 +17,13 @@ Implicit Types σ : state.
 
 Definition zebre_adequacy Σ `{zebre_Gpre : !ZebreGpre Σ} e σ :
   ( ∀ `{zebre_G : !ZebreG Σ},
-    ⊢ WP e @ ⊤ {{ v, True }}
+    ⊢ WP e {{ v, True }}
   ) →
   adequate e σ.
 Proof.
   intros Hwp.
   apply: wp_adequacy => Hinv_G κs.
-  iMod zebre_init as "(%zebre_G & Hσ)".
-  iExists zebre_state_interp, (λ _, True%I), _. iFrame.
+  iMod zebre_init' as "(%zebre_G & Hσ)".
+  iExists zebre_state_interp. repeat iExists _. iFrame.
   iApply (Hwp (Build_ZebreG Σ)).
 Qed.
